src/high/resources/gen_predicates.v
@@ -21,7 +21,7 @@ Definition predicatesR Σ := authR (gmapUR loc (predicateR Σ)).
 Notation predicates_inG Σ Ω := (genInDepsG Σ Ω (predicatesR Σ) [#crashed_atR]).
 
 Section ownership.
-  Context `{!nvmBaseG Σ Ω, !predicates_inG Σ Ω}.
+  Context `{!nvmBaseGS Σ Ω, !predicates_inG Σ Ω}.
   Implicit Type (OCV: view) (PRs: gmap loc (predicateR Σ)) (PR: predicateR Σ).
 
   (* TODO: both this definition and the lemma below are duplicates *)
